SCCAlg.v
@@ -57,62 +57,11 @@ Qed.
 Module D1 := (D O S G F).
 Module Der1 := (DerivedProofs.DerivedProofs O S G F D1).
 
-(*Finding the minimum element in a list based on a given function (needed to find vertex with smallest
-  discovery time in SCC*)
-Definition min_elt_list (l: list O.t) (f: O.t -> nat) : option O.t :=
-  fold_right (fun x s => match s with
-                     | None => Some x
-                     | Some y =>  if (f x <? f y) then Some x else s
-                     end) None l.
+Module M := (Helper.MinMax O).
+Import M.
 
 Definition min_elt_set (c: S.t) (f: O.t -> nat) : option O.t:=
   min_elt_list (S.elements c) f.
-
-Lemma min_elt_list_none_iff_empty: forall l f,
-  min_elt_list l f = None <-> l = nil.
-Proof.
-  intros. induction l; simpl in *; split; intros; try(reflexivity).
-  - destruct (min_elt_list l f) eqn : ?.
-    + destruct (f a <? f t); inversion H.
-    + inversion H.
-  - inversion H.
-Qed.
-
-Lemma min_elt_list_in_list: forall f x l,
-  min_elt_list l f = Some x ->
-  In x l.
-Proof.
-  intros. generalize dependent x. induction l; intros.
-  - simpl in H. inversion H.
-  - simpl in *. destruct (min_elt_list l f) eqn : ?.
-    + destruct (f a <? f t) eqn : ?; inversion H; subst. left. reflexivity. right. apply IHl.
-      reflexivity.
-    + inversion H; subst. left. reflexivity.
-Qed.
-
-Lemma min_elt_list_finds_min: forall f x l,
-  (forall x y, In x l -> In y l -> f x = f y -> x = y) ->
-  min_elt_list l f = Some x ->
-  forall y, In y l -> y <> x -> f x < f y.
-Proof.
-  intros. generalize dependent x. induction l; intros.
-  - destruct H1.
-  - simpl in H1. simpl in H0. destruct H1.
-    + subst. destruct (min_elt_list l f ) eqn : ?.
-      * destruct (f y <? f t ) eqn : ?.
-        -- inversion H0; subst. contradiction.
-        -- inversion H0; subst.  rewrite Nat.ltb_antisym in Heqb. simplify.
-        rewrite Nat.leb_le in Heqb. assert (f x < f y \/ f x = f y) by omega.
-        destruct H1. apply H1. apply H in H1. subst. contradiction. simpl. right.
-        eapply  min_elt_list_in_list. apply Heqo. left. reflexivity.
-      * inversion H0; subst. contradiction.
-    + destruct (min_elt_list l f) eqn : ?. destruct (f a <? f t ) eqn : ?.
-      * rewrite Nat.ltb_lt in Heqb. inversion H0; subst. destruct (O.eq_dec t y). unfold O.eq in e.
-        subst. apply Heqb. assert (f t < f y). apply IHl. intros. apply H; try(solve_in).
-        apply H1. reflexivity. auto. omega.
-      * inversion H0; subst.  rewrite Nat.ltb_antisym in Heqb. simplify.
-      * inversion H0; subst. rewrite min_elt_list_none_iff_empty in Heqo. subst. inversion H1.
-Qed.
 
 Lemma min_elt_set_none_iff_empty: forall s f,
   min_elt_set s f = None <-> S.is_empty s = true.
@@ -155,62 +104,9 @@ Qed.
 Definition d_time_scc g c (H: scc c g) :=
   min_elt_set c (D1.d_time None g).
 
-(*The same but for max/finish time*)
-
-Definition max_elt_list (l: list O.t) (f: O.t -> nat) : option O.t :=
-  fold_right (fun x s => match s with
-                     | None => Some x
-                     | Some y =>  if (f y <? f x) then Some x else s
-                     end) None l.
-
 Definition max_elt_set (c: S.t) (f: O.t -> nat) : option O.t:=
   max_elt_list (S.elements c) f.
 
-Lemma max_elt_list_none_iff_empty: forall l f,
-  max_elt_list l f = None <-> l = nil.
-Proof.
-  intros. induction l; simpl in *; split; intros; try(reflexivity).
-  - destruct (max_elt_list l f) eqn : ?.
-    + destruct (f t <? f a); inversion H.
-    + inversion H.
-  - inversion H.
-Qed.
-
-Lemma max_elt_list_in_list: forall f x l,
-  max_elt_list l f = Some x ->
-  In x l.
-Proof.
-  intros. generalize dependent x. induction l; intros.
-  - simpl in H. inversion H.
-  - simpl in *. destruct (max_elt_list l f) eqn : ?.
-    + destruct (f t <? f a) eqn : ?; inversion H; subst. left. reflexivity. right. apply IHl.
-      reflexivity.
-    + inversion H; subst. left. reflexivity.
-Qed.
-
-Lemma max_elt_list_finds_max: forall f x l,
-  (forall x y, In x l -> In y l -> f x = f y -> x = y) ->
-  max_elt_list l f = Some x ->
-  forall y, In y l -> y <> x -> f y < f x.
-Proof.
-  intros. generalize dependent x. induction l; intros.
-  - destruct H1.
-  - simpl in H1. simpl in H0. destruct H1.
-    + subst. destruct (max_elt_list l f ) eqn : ?.
-      * destruct (f t <? f y ) eqn : ?.
-        -- inversion H0; subst. contradiction.
-        -- inversion H0; subst.  rewrite Nat.ltb_antisym in Heqb. simplify.
-        rewrite Nat.leb_le in Heqb. assert (f y < f x \/ f y = f x) by omega.
-        destruct H1. apply H1. apply H in H1. subst. contradiction. left. reflexivity.
-        right. eapply max_elt_list_in_list. apply Heqo.
-      * inversion H0; subst. contradiction.
-    + destruct (max_elt_list l f) eqn : ?. destruct (f t <? f a ) eqn : ?.
-      * rewrite Nat.ltb_lt in Heqb. inversion H0; subst. destruct (O.eq_dec t y). unfold O.eq in e.
-        subst. apply Heqb. assert (f y < f t). apply IHl. intros. apply H; try(solve_in). apply H1.
-        reflexivity. auto. omega.
-      * inversion H0; subst.  rewrite Nat.ltb_antisym in Heqb. simplify.
-      * inversion H0; subst. rewrite max_elt_list_none_iff_empty in Heqo. subst. inversion H1.
-Qed.
 
 Lemma max_elt_set_none_iff_empty: forall s f,
   max_elt_set s f = None <-> S.is_empty s = true.
@@ -621,77 +517,7 @@ Proof.
         eapply get_tree_in_graph. apply R1. assumption.
 Qed. 
 
-(** Finding the minimum element of a path **)
-(*Because a path has the start, end, and intermediate list, this basically boils down to a ton of cases*)
-
-Definition min_elt_path (u v : O.t) (f: O.t -> nat) l :=
-  match (min_elt_list l f) with
-  | Some x => if f u <? f x then 
-                if f u <? f v then u 
-                else v
-             else if f v <? f x then v else x
-  | None => if f u <? f v then u else v
-  end.
-
-Ltac destruct_if := 
-  match goal with
-  | [H : (if ?a <? ?b then _ else _) = _ |- _ ] => (destruct (a <? b) eqn : ?)
-  end.
-
-Lemma min_elt_path_in: forall u v l f x,
-  min_elt_path u v f l = x ->
-  x = u \/ x = v \/ In x l.
-Proof.
-  intros. unfold min_elt_path in H. destruct (min_elt_list l f) eqn : ?.
-  repeat(destruct_if; try(simplify)). subst.
-  right. right. apply min_elt_list_in_list in Heqo. assumption.
-  destruct_if; inversion H; simplify.
-Qed.
-
-Lemma min_elt_path_finds_min: forall u v l f x,
-  (forall x0 y0 : O.t, (u = x0 \/ v = x0 \/ In x0 l) -> (u = y0 \/ v = y0 \/ In y0 l) -> f x0 = f y0 -> x0 = y0) ->
-  ~In u l -> ~In v l -> u <> v ->
-  min_elt_path u v f l = x ->
-  (forall y, y = u \/ y = v \/ In y l -> y <> x -> f x < f y).
-Proof.
-  intros. unfold min_elt_path in H3. destruct (min_elt_list l f) eqn : ?.
-  repeat((destruct_if); repeat(rewrite Nat.ltb_lt in *)); subst.
-  simplify; subst; try(assumption); try(omega). destruct (O.eq_dec y t). unfold O.eq in e. subst.
-  assumption. eapply min_elt_list_finds_min in Heqo. assert (f t < f y) by apply Heqo. omega.
-  intros; apply H; try(right; right; assumption); assumption. apply H4. auto.
-  assert (f x < f u). { rewrite Nat.ltb_antisym in Heqb0. rewrite negb_false_iff in Heqb0.
-  apply Nat.leb_le in Heqb0. assert ( f x < f u \/ f x = f u) by omega. destruct H3. apply H3.
-  apply H in H3. subst. contradiction. right. left. reflexivity. left. reflexivity. }
-  clear Heqb0. simplify; subst; try(assumption); try(omega).
-  destruct (O.eq_dec t y). unfold O.eq in e. subst. omega. eapply min_elt_list_finds_min in Heqo.
-  assert (f t < f y) by apply Heqo. omega. intros; apply H; try(right; right; assumption); assumption. 
-  apply H4. auto. assert (f t < f u). { rewrite Nat.ltb_antisym in Heqb. rewrite negb_false_iff in Heqb.
-  apply Nat.leb_le in Heqb. assert (f t < f u \/ f t = f u) by omega. destruct H3.
-  apply H3. subst. eapply H in H3. subst. apply min_elt_list_in_list in Heqo. contradiction.
-  right. right. apply min_elt_list_in_list in Heqo; assumption. left. reflexivity. }
-  clear Heqb.  simplify; subst; try(assumption); try(omega). destruct (O.eq_dec y t). unfold O.eq in e.
-  subst. omega. eapply min_elt_list_finds_min in Heqo. assert (f t < f y) by apply Heqo. omega.
-  intros; apply H; try(right; right; assumption); assumption.  apply H4. auto.
-  assert ( f x < f v). { rewrite Nat.ltb_antisym in Heqb0. rewrite negb_false_iff in Heqb0.
-  apply Nat.leb_le in Heqb0. assert ( f x < f v \/ f x = f v) by omega. destruct H3. apply H3.
-  apply H in H3. subst. apply min_elt_list_in_list in Heqo. contradiction. right. right.
-  eapply min_elt_list_in_list. apply Heqo. right. left. reflexivity. } clear Heqb0.
-  assert ( f x < f u). { rewrite Nat.ltb_antisym in Heqb. rewrite negb_false_iff in Heqb.
-  apply Nat.leb_le in Heqb. assert (f x < f u \/ f x = f u) by omega. destruct H6.
-  apply H6. subst. eapply H in H6. subst. apply min_elt_list_in_list in Heqo. contradiction.
-  right. right. apply min_elt_list_in_list in Heqo; assumption. left. reflexivity. }
-  clear Heqb. simplify; subst; try(assumption); try(omega).
-  eapply min_elt_list_finds_min in Heqo. apply Heqo.  intros; apply H; try(right; right; assumption).
-  assumption. assumption. auto. destruct_if; repeat( rewrite Nat.ltb_lt in *); subst.
-  simplify; subst; try(assumption); try(omega). apply min_elt_list_none_iff_empty in Heqo. subst.
-  inversion H4. assert (f x < f u). { rewrite Nat.ltb_antisym in Heqb. rewrite negb_false_iff in Heqb.
-  apply Nat.leb_le in Heqb. assert ( f x < f u \/ f x = f u) by omega. destruct H3. apply H3.
-  apply H in H3. subst. contradiction. right. left. reflexivity. left. reflexivity. }
-  clear Heqb. simplify; subst; try(assumption); try(omega).  
-  apply min_elt_list_none_iff_empty in Heqo. subst. inversion H4.
-Qed.
-
-(*Why we cared about this: every path has a vertex along it that was discovered first*)
+(*Every path has a vertex along it that was discovered first*)
 Lemma path_has_first_discovered: forall g u v l lt H,
   Pa.path_list_rev g u v l = true ->
   NoDup l -> ~In u l -> ~In v l ->
